Should all be fixed up

example.c
@@ -10,10 +10,10 @@ void publish(int x) {
 }
 
 int main() {
-	int secret = 5;
-	int sensitive[4] = {0,0,0,0};
 	int (*foo)() = f;
 	int res = (*foo)();
+	int secret = 5;
+	int sensitive[4] = {0,0,0,0};
 	if (sensitive[0] == 42)
 		publish(secret);
 	else
