tests/stack_load_store_ib.c
@@ -1,0 +1,9 @@
+int main() {
+	int x[3];
+
+	for (int i = 0; i < 3; i++) {
+		x[i] = i;
+	}
+
+	return x[0];
+}
